Phi_Semantics_Framework/Phi_Semantics_Framework.thy
@@ -248,38 +248,38 @@ subsection \<open>Formalization of Computation\<close>
 
 subsubsection \<open>Explicit Annotation of Semantic Arguments and Returns\<close>
 
-text \<open>Arguments and Returns are wrapped by sem type.
-  For sure this wrap is not necessary, but it helps the programming framework and syntax parser
-  to recognize which entity is an argument or a return.\<close>
+text \<open>Arguments and Returns are wrapped by \<phi>arg type.
+  It helps the programming framework and syntax parser to recognize which one is an argument
+  or a return, among values that may be used for other purposes of specification.\<close>
 
-datatype ('a::VALs) sem = sem (dest: 'a)
+datatype ('a::VALs) \<phi>arg = \<phi>arg (dest: 'a)
 hide_const (open) dest
 
 
-lemma sem_value_forall: \<open>All P \<longleftrightarrow> (\<forall>x. P (sem x))\<close> by (metis sem.exhaust)
-lemma sem_value_exists: \<open>Ex P  \<longleftrightarrow> (\<exists>x. P (sem x))\<close> by (metis sem.exhaust)
-lemma sem_value_All: \<open>(\<And>x. PROP P x) \<equiv> (\<And>x. PROP P (sem x))\<close>
+lemma sem_value_forall: \<open>All P \<longleftrightarrow> (\<forall>x. P (\<phi>arg x))\<close> by (metis \<phi>arg.exhaust)
+lemma sem_value_exists: \<open>Ex P  \<longleftrightarrow> (\<exists>x. P (\<phi>arg x))\<close> by (metis \<phi>arg.exhaust)
+lemma sem_value_All: \<open>(\<And>x. PROP P x) \<equiv> (\<And>x. PROP P (\<phi>arg x))\<close>
 proof
-  fix x :: 'a assume A: \<open>(\<And>x. PROP P x)\<close> then show \<open>PROP P (sem x)\<close> .
+  fix x :: 'a assume A: \<open>(\<And>x. PROP P x)\<close> then show \<open>PROP P (\<phi>arg x)\<close> .
 next
-  fix x :: \<open>'a sem\<close> assume A: \<open>\<And>x. PROP P (sem x)\<close>
-  from \<open>PROP P (sem (sem.dest x))\<close> show "PROP P x" by simp
+  fix x :: \<open>'a \<phi>arg\<close> assume A: \<open>\<And>x. PROP P (\<phi>arg x)\<close>
+  from \<open>PROP P (\<phi>arg (\<phi>arg.dest x))\<close> show "PROP P x" by simp
 qed
 
-abbreviation \<open>\<phi>V_none \<equiv> sem ()\<close>
-definition \<open>\<phi>V_pair x y = sem (sem.dest x, sem.dest y)\<close>
-definition \<open>\<phi>V_fst x = map_sem fst x\<close>
-definition \<open>\<phi>V_snd x = map_sem snd x\<close>
-abbreviation \<open>\<phi>V_nil \<equiv> sem []\<close>
-definition \<open>\<phi>V_cons h l = sem (sem.dest h # sem.dest l)\<close>
-definition \<open>\<phi>V_hd l = sem (hd (sem.dest l))\<close>
-definition \<open>\<phi>V_tl l = sem (tl (sem.dest l))\<close>
+abbreviation \<open>\<phi>V_none \<equiv> \<phi>arg ()\<close>
+definition \<open>\<phi>V_pair x y = \<phi>arg (\<phi>arg.dest x, \<phi>arg.dest y)\<close>
+definition \<open>\<phi>V_fst x = map_\<phi>arg fst x\<close>
+definition \<open>\<phi>V_snd x = map_\<phi>arg snd x\<close>
+abbreviation \<open>\<phi>V_nil \<equiv> \<phi>arg []\<close>
+definition \<open>\<phi>V_cons h l = \<phi>arg (\<phi>arg.dest h # \<phi>arg.dest l)\<close>
+definition \<open>\<phi>V_hd l = \<phi>arg (hd (\<phi>arg.dest l))\<close>
+definition \<open>\<phi>V_tl l = \<phi>arg (tl (\<phi>arg.dest l))\<close>
 
 lemma \<phi>V_simps[simp]:
   \<open>\<phi>V_pair (\<phi>V_fst v) (\<phi>V_snd v) = v\<close>
   \<open>\<phi>V_fst (\<phi>V_pair u y) = u\<close>
   \<open>\<phi>V_snd (\<phi>V_pair x u) = u\<close>
-  \<open>\<phi>V_cons (sem h) (sem l) = sem (h#l)\<close>
+  \<open>\<phi>V_cons (\<phi>arg h) (\<phi>arg l) = \<phi>arg (h#l)\<close>
   \<open>\<phi>V_hd (\<phi>V_cons hv lv) = hv\<close>
   \<open>\<phi>V_tl (\<phi>V_cons hv lv) = lv\<close>
   unfolding \<phi>V_pair_def \<phi>V_fst_def \<phi>V_snd_def \<phi>V_cons_def \<phi>V_hd_def \<phi>V_tl_def
@@ -338,7 +338,7 @@ text \<open>\<open>('ret,'ex,'RES_N,'RES) state\<close> represents any potential
 declare [ [typedef_overloaded] ]
 
 datatype 'ret state =
-      Success \<open>'ret::VALs sem\<close> (resource: resource)
+      Success \<open>'ret::VALs \<phi>arg\<close> (resource: resource)
     | Exception \<open>ABNM\<close> (resource: resource)
     | Invalid | PartialCorrect
 
@@ -392,7 +392,7 @@ is expressed by returning \<open>Invalid\<close>.
  \<close>
 
 type_synonym 'ret proc = "resource \<Rightarrow> 'ret state set"
-type_synonym ('arg,'ret) proc' = "'arg sem \<Rightarrow> 'ret proc"
+type_synonym ('arg,'ret) proc' = "'arg \<phi>arg \<Rightarrow> 'ret proc"
 
 
 definition bind :: "'a::VALs proc \<Rightarrow> ('a,'b) proc' \<Rightarrow> 'b::VALs proc"  ("_ \<bind>/ _" [75,76] 75)
