Phi_System/Calculus_of_Programming.thy
@@ -50,7 +50,7 @@ abbreviation View_Shift_CurrentConstruction ("\<^bold>v\<^bold>i\<^bold>e\<^bold
 definition PendingConstruction :: " 'ret::VALs proc
                                   \<Rightarrow> resource
                                   \<Rightarrow> assn
-                                  \<Rightarrow> ('ret sem \<Rightarrow> assn)
+                                  \<Rightarrow> ('ret \<phi>arg \<Rightarrow> assn)
                                   \<Rightarrow> (ABNM \<Rightarrow> assn)
                                   \<Rightarrow> bool "
     ("\<^bold>p\<^bold>e\<^bold>n\<^bold>d\<^bold>i\<^bold>n\<^bold>g _ \<^bold>o\<^bold>n _ [_]/ \<^bold>r\<^bold>e\<^bold>s\<^bold>u\<^bold>l\<^bold>t\<^bold>s \<^bold>i\<^bold>n _/ \<^bold>t\<^bold>h\<^bold>r\<^bold>o\<^bold>w\<^bold>s _" [1000,1000,1000,11,11] 10)
@@ -121,7 +121,7 @@ lemma \<phi>accept_proc_optimize_\<phi>V_none:
 (*
 lemma \<phi>return_when_unreachable:
   \<open> \<^bold>p\<^bold>e\<^bold>n\<^bold>d\<^bold>i\<^bold>n\<^bold>g f \<^bold>o\<^bold>n s [R] \<^bold>r\<^bold>e\<^bold>s\<^bold>u\<^bold>l\<^bold>t\<^bold>s \<^bold>i\<^bold>n (\<lambda>_. T) \<^bold>t\<^bold>h\<^bold>r\<^bold>o\<^bold>w\<^bold>s E
-\<Longrightarrow> \<^bold>p\<^bold>e\<^bold>n\<^bold>d\<^bold>i\<^bold>n\<^bold>g (f \<ggreater> Return (sem undefined)) \<^bold>o\<^bold>n s [R] \<^bold>r\<^bold>e\<^bold>s\<^bold>u\<^bold>l\<^bold>t\<^bold>s \<^bold>i\<^bold>n (\<lambda>_. T) \<^bold>t\<^bold>h\<^bold>r\<^bold>o\<^bold>w\<^bold>s E\<close>
+\<Longrightarrow> \<^bold>p\<^bold>e\<^bold>n\<^bold>d\<^bold>i\<^bold>n\<^bold>g (f \<ggreater> Return (\<phi>arg undefined)) \<^bold>o\<^bold>n s [R] \<^bold>r\<^bold>e\<^bold>s\<^bold>u\<^bold>l\<^bold>t\<^bold>s \<^bold>i\<^bold>n (\<lambda>_. T) \<^bold>t\<^bold>h\<^bold>r\<^bold>o\<^bold>w\<^bold>s E\<close>
   for f :: \<open>unreachable proc\<close>
   unfolding CurrentConstruction_def PendingConstruction_def bind_def Return_def det_lift_def subset_iff
   apply clarsimp subgoal for s' s'' by (cases s'; simp; cases s''; simp add: ring_distribs; blast) .
@@ -149,7 +149,7 @@ lemma \<phi>reassemble_proc_final:
 
 lemma "\<phi>__Return_rule__":
   \<open> \<^bold>v\<^bold>i\<^bold>e\<^bold>w X \<longmapsto> Y \<^bold>w\<^bold>i\<^bold>t\<^bold>h Any
-\<Longrightarrow> \<^bold>p\<^bold>r\<^bold>o\<^bold>c Return \<phi>V_none \<lbrace> X \<longmapsto> \<lambda>_::unit sem. Y \<rbrace>\<close>
+\<Longrightarrow> \<^bold>p\<^bold>r\<^bold>o\<^bold>c Return \<phi>V_none \<lbrace> X \<longmapsto> \<lambda>_::unit \<phi>arg. Y \<rbrace>\<close>
   unfolding \<phi>Procedure_def Return_def View_Shift_def subset_iff det_lift_def
   by clarsimp
 
@@ -361,7 +361,7 @@ paragraph \<open>Return\<close>
 
 lemma \<phi>M_Success[intro!]:
   \<open> v \<in> (y \<Ztypecolon> T)
-\<Longrightarrow> \<^bold>p\<^bold>r\<^bold>o\<^bold>c Return (sem v) \<lbrace> X \<longmapsto> \<lambda>u. X\<heavy_comma> y \<Ztypecolon> Val u T \<rbrace> \<^bold>t\<^bold>h\<^bold>r\<^bold>o\<^bold>w\<^bold>s Any \<close>
+\<Longrightarrow> \<^bold>p\<^bold>r\<^bold>o\<^bold>c Return (\<phi>arg v) \<lbrace> X \<longmapsto> \<lambda>u. X\<heavy_comma> y \<Ztypecolon> Val u T \<rbrace> \<^bold>t\<^bold>h\<^bold>r\<^bold>o\<^bold>w\<^bold>s Any \<close>
   unfolding \<phi>Procedure_def det_lift_def Return_def
   by (clarsimp simp add: \<phi>expns)
 
